tests/ThemiPraxis/ThemiPraxis_Smoke.v
@@ -1,4 +1,4 @@
-﻿From Coq Require Import Program Setoids.Setoid.
+From Coq Require Import Program Setoids.Setoid.
 
 (* Standalone definitions for compilation - using PXL canonical model types *)
 Parameter form : Type.
@@ -17,51 +17,51 @@ Class Euclidean : Prop := { euclidean_R : forall w u v, can_R w u -> can_R w v -
 Class Serial : Prop := { serial_R : forall w, exists v, can_R w v }.
 
 (* Theorems from ModalPraxis *)
-Parameter provable_K : forall φ ψ, Prov (Impl (Box (Impl φ ψ)) (Impl (Box φ) (Box ψ))).
-Parameter provable_necessitation : forall φ, (forall w, forces w φ) -> Prov (Box φ).
-Parameter provable_D : Serial -> forall φ, Prov (Impl (Box φ) (Dia φ)).
-Parameter provable_4 : Transitive -> forall φ, Prov (Impl (Box φ) (Box (Box φ))).
-Parameter provable_5 : Euclidean -> forall φ, Prov (Impl (Dia φ) (Box (Dia φ))).
+Parameter provable_K : forall f g, Prov (Impl (Box (Impl f g)) (Impl (Box f) (Box g))).
+Parameter provable_necessitation : forall f, (forall w, forces w f) -> Prov (Box f).
+Parameter provable_D : Serial -> forall f, Prov (Impl (Box f) (Dia f)).
+Parameter provable_4 : Transitive -> forall f, Prov (Impl (Box f) (Box (Box f))).
+Parameter provable_5 : Euclidean -> forall f, Prov (Impl (Dia f) (Box (Dia f))).
 
 Module ThemiPraxis.
 
-  (* Worlds already provided by kernel; we use modal □ as "Obligatory". *)
-  Definition O (φ:form) : form := Box φ.
-  Definition P (φ:form) : form := Dia φ.  (* Permitted *)
+  (* Worlds already provided by kernel; we use modal ? as "Obligatory". *)
+  Definition O (f:form) : form := Box f.
+  Definition P (f:form) : form := Dia f.  (* Permitted *)
 
   (* Frame classes for deontic systems *)
   Class K_Frame  : Prop := {}.                         (* base normal *)
-  Class KD_Frame : Prop := { kd_serial : Serial }.     (* D: Oφ → Pφ *)
+  Class KD_Frame : Prop := { kd_serial : Serial }.     (* D: Of ? Pf *)
   Class KD45_Frame : Prop := { kd_serial' : Serial; kd_trans : Transitive; kd_eucl : Euclidean }.
 
   (* Base normal rules *)
-  Theorem K_axiom : K_Frame -> forall φ ψ, Prov (Impl (O (Impl φ ψ)) (Impl (O φ) (O ψ))).
-  Proof. intros _ φ ψ; change (Prov (Impl (Box (Impl φ ψ)) (Impl (Box φ) (Box ψ)))); apply provable_K. Qed.
+  Theorem K_axiom : K_Frame -> forall f g, Prov (Impl (O (Impl f g)) (Impl (O f) (O g))).
+  Proof. intros _ f g; change (Prov (Impl (Box (Impl f g)) (Impl (Box f) (Box g)))); apply provable_K. Qed.
 
-  Theorem Necessitation : K_Frame -> forall φ, (forall w, forces w φ) -> Prov (O φ).
-  Proof. intros _ φ H; change (Prov (Box φ)); apply provable_necessitation; exact H. Qed.
+  Theorem Necessitation : K_Frame -> forall f, (forall w, forces w f) -> Prov (O f).
+  Proof. intros _ f H; change (Prov (Box f)); apply provable_necessitation; exact H. Qed.
 
   (* D: seriality *)
-  Theorem D_axiom : KD_Frame -> forall φ, Prov (Impl (O φ) (P φ)).
-  Proof. intros H φ; destruct H as [Hser]; change (Prov (Impl (Box φ) (Dia φ))); eapply provable_D; eauto. Qed.
+  Theorem D_axiom : KD_Frame -> forall f, Prov (Impl (O f) (P f)).
+  Proof. intros H f; destruct H as [Hser]; change (Prov (Impl (Box f) (Dia f))); eapply provable_D; eauto. Qed.
 
   (* 4 and 5 under KD45; standard KD45 deontic *)
-  Theorem Four_axiom : KD45_Frame -> forall φ, Prov (Impl (O φ) (O (O φ))).
-  Proof. intros H φ; destruct H as [Hs Ht He]; change (Prov (Impl (Box φ) (Box (Box φ)))); eapply provable_4; eauto. Qed.
+  Theorem Four_axiom : KD45_Frame -> forall f, Prov (Impl (O f) (O (O f))).
+  Proof. intros H f; destruct H as [Hs Ht He]; change (Prov (Impl (Box f) (Box (Box f)))); eapply provable_4; eauto. Qed.
 
-  Theorem Five_axiom : KD45_Frame -> forall φ, Prov (Impl (P φ) (O (P φ))).
-  Proof. intros H φ; destruct H as [Hs Ht He]; change (Prov (Impl (Dia φ) (Box (Dia φ)))); eapply provable_5; eauto. Qed.
+  Theorem Five_axiom : KD45_Frame -> forall f, Prov (Impl (P f) (O (P f))).
+  Proof. intros H f; destruct H as [Hs Ht He]; change (Prov (Impl (Dia f) (Box (Dia f)))); eapply provable_5; eauto. Qed.
 
 End ThemiPraxis.
 
 Module T.
   Import ThemiPraxis.
-  Lemma k_ok  : K_Frame  -> forall φ ψ, Prov (Impl (O (Impl φ ψ)) (Impl (O φ) (O ψ))).
+  Lemma k_ok  : K_Frame  -> forall f g, Prov (Impl (O (Impl f g)) (Impl (O f) (O g))).
   Proof. apply K_axiom. Qed.
-  Lemma d_ok  : KD_Frame -> forall φ, Prov (Impl (O φ) (P φ)).
+  Lemma d_ok  : KD_Frame -> forall f, Prov (Impl (O f) (P f)).
   Proof. apply D_axiom. Qed.
-  Lemma d45_4_ok : KD45_Frame -> forall φ, Prov (Impl (O φ) (O (O φ))).
+  Lemma d45_4_ok : KD45_Frame -> forall f, Prov (Impl (O f) (O (O f))).
   Proof. apply Four_axiom. Qed.
-  Lemma d45_5_ok : KD45_Frame -> forall φ, Prov (Impl (P φ) (O (P φ))).
+  Lemma d45_5_ok : KD45_Frame -> forall f, Prov (Impl (P f) (O (P f))).
   Proof. apply Five_axiom. Qed.
 End T.
