modules/IEL/experimental/ChremaPraxis/theorems/Systems.v
@@ -1,2 +1,2 @@
-﻿From Coq Require Import Program Setoids.Setoid.
+From Coq Require Import Program Setoids.Setoid.
 Module ChremaPraxisSystem. End ChremaPraxisSystem.
