modules/IEL/experimental/HexiPraxis/theorems/NormalBase.v
@@ -1,3 +1,3 @@
-﻿From Coq Require Import Program Setoids.Setoid.
+From Coq Require Import Program Setoids.Setoid.
 Set Implicit Arguments.
 (* HexiPraxis NormalBase  core rules placeholder; keep constructive. *)
