modules/IEL/experimental/MuPraxis/modal/FrameSpec.v
@@ -1,3 +1,3 @@
-﻿From Coq Require Import Program Setoids.Setoid.
+From Coq Require Import Program Setoids.Setoid.
 Set Implicit Arguments.
 (* MuPraxis FrameSpec  interface placeholder; fill with relations/flags for MuPraxis. *)
