modules/IEL/experimental/MuPraxis/theorems/Conservativity.v
@@ -1,3 +1,3 @@
-﻿From Coq Require Import Program.
+From Coq Require Import Program.
 (* From PXLs Require Import PXLv3. *)
 Goal True. exact I. Qed.
