modules/IEL/experimental/MuPraxis/theorems/NormalBase.v
@@ -1,4 +1,4 @@
-﻿From Coq Require Import Program.
+From Coq Require Import Program.
 (* From PXLs Require Import PXLv3.
 Require Import modules.IEL.MuPraxis.modal.FixSpec. *)
 Set Implicit Arguments.
