modules/IEL/modal/FrameSpec.v
@@ -1,4 +1,0 @@
-From Coq Require Import Program.
-From PXLs Require Import PXLv3.
-Set Implicit Arguments.
-(*  FrameSpec  interface placeholder; fill with relations/flags for . *)
