tests/TropoPraxis/TropoPraxis_Smoke.v
@@ -1,2 +1,2 @@
-﻿From Coq Require Import Program Setoids.Setoid.
+From Coq Require Import Program Setoids.Setoid.
 Goal True. exact I. Qed.
